adding current working state

intermediate/Veritas.Intermediate.VerifyS.fst
@@ -494,32 +494,6 @@ let lemma_vevictbm_preserves_inv
           (ensures (store_inv (thread_store (vevictbm s s' t vs))))
   = () // TODO: VERY suspicious
 
-(* This is basically a "light" version of the vfun functions to reconstruct the log. 
-   We could have the vfun functions return logK entries instead, but this seems cleaner. *)
-let logS_to_logK_entry (vs:vtls{Valid? vs}) (e:logS_entry) : option logK_entry =
-  let st = thread_store vs in
-  match e with
-  | Get_S s k v -> 
-      if store_contains st s && k = stored_key st s
-      then Some (Spec.Get k v) else None
-  | Put_S s k v -> 
-      if store_contains st s && k = stored_key st s
-      then Some (Spec.Put k v) else None
-  | AddM_S _ r s' -> 
-      if store_contains st s' && is_merkle_key (stored_key st s') 
-      then Some (Spec.AddM r (stored_key st s')) else None
-  | EvictM_S s s' -> 
-      if store_contains st s && store_contains st s' && is_merkle_key (stored_key st s') 
-      then Some (Spec.EvictM (stored_key st s) (stored_key st s')) else None
-  | AddB_S _ r t j -> 
-      Some (Spec.AddB r t j)
-  | EvictB_S s t -> 
-      if store_contains st s
-      then Some (Spec.EvictB (stored_key st s) t) else None
-  | EvictBM_S s s' t ->
-      if store_contains st s && store_contains st s' && is_merkle_key (stored_key st s') 
-      then Some (Spec.EvictBM (stored_key st s) (stored_key st s') t) else None
-
 let lemma_t_verify_step_valid_implies_log_exists (vs:vtls) (e:logS_entry)
   : Lemma (requires (Valid? (t_verify_step vs e)))
           (ensures (Some? (logS_to_logK_entry vs e)))
@@ -549,7 +523,34 @@ let lemma_init_thread_state_rel (id:thread_id)
       let st' = Spec.thread_store vs' in
       lemma_store_rel_add_to_store st st' 0 Root (init_value Root) Spec.MAdd
 
-let get_log (vs:vtls) (l:logS{Valid? (fst (t_verify_aux vs l))}) : logK
+let adds_duplicate_key (st:vstore) (e:logS_entry)
+  = match e with
+    | AddM_S _ (k,_) _ -> store_contains_key st k
+    | AddB_S _ (k,_) _ _ -> store_contains_key st k
+    | _ -> false
+
+(* If the output state is Valid and the store satisfies store_inv, then the intermediate-level
+   state after one step is related to the spec-level state. Note that we can't say anything 
+   stronger (e.g. t_verify simulates Spec.t_verify) without more restrictive preconditions. 
+   (The statement below does not guarantee that the result preserves store_inv.) *)
+let lemma_t_verify_step_simulates_spec (vs:vtls) (vs':Spec.vtls) (e:logS_entry)
+  : Lemma (requires (vtls_rel vs vs' /\ 
+                     Valid? (t_verify_step vs e) /\
+                     not (adds_duplicate_key (thread_store vs) e) /\
+                     store_inv (thread_store vs)))
+          (ensures (vtls_rel (t_verify_step vs e) 
+                             (Spec.t_verify_step vs' (Some?.v (logS_to_logK_entry vs e)))))
+  = let st = thread_store vs in
+    match e with
+    | Get_S s k v -> lemma_vget_simulates_spec vs vs' s k v
+    | Put_S s k v -> lemma_vput_simulates_spec vs vs' s k v
+    | AddM_S s r s' -> lemma_vaddm_simulates_spec_if_k_is_new vs vs' s s' r (stored_key st s')
+    | EvictM_S s s' -> lemma_vevictm_simulates_spec vs vs' s s' (stored_key st s) (stored_key st s')
+    | AddB_S s r t j -> lemma_vaddb_simulates_spec_if_k_is_new vs vs' s r t j
+    | EvictB_S s t -> lemma_vevictb_simulates_spec vs vs' s (stored_key st s) t
+    | EvictBM_S s s' t -> lemma_vevictbm_simulates_spec vs vs' s s' (stored_key st s) (stored_key st s') t
+
+(*let get_log (vs:vtls) (l:logS{Valid? (fst (t_verify_aux vs l))}) : logK
   = Some?.v (snd (t_verify_aux vs l))
 
 let rec lemma_get_log_length (vs:vtls) (l:logS)
@@ -568,35 +569,6 @@ let lemma_get_log_prefix_commute (vs:vtls) (l:logS)
           (ensures (let n = Seq.length l in
                     Seq.equal (get_log vs (prefix l (n - 1))) (prefix (get_log vs l) (n - 1))))
   = ()
-
-(*
-let rec lemma_t_verify_aux_simulates_spec (vs:vtls) (vs':Spec.vtls) (l:logS)
-  : Lemma (requires (vtls_rel vs vs' /\ Valid? (fst (t_verify_aux vs l))))
-          (ensures (let res = t_verify_aux vs l in
-                    vtls_rel (fst res) (Spec.t_verify_aux vs' (Some?.v (snd res)))))
-          (decreases (Seq.length l))
-  = let n = Seq.length l in
-    if n <> 0
-    then
-      let lp = prefix l (n - 1) in
-      let e = Seq.index l (n - 1) in
-      let (vsp,lp') = t_verify_aux vs lp in
-      if Valid? vsp
-      then (
-        lemma_t_verify_aux_simulates_spec vs vs' lp; // I.H.
-        let vsp' = Spec.t_verify_aux vs' (Some?.v lp') in
-        lemma_get_log_prefix_commute vs l;
-        if thread_store_is_map vsp
-        then lemma_t_verify_step_simulates_spec1 vsp vsp' e
-        else lemma_t_verify_step_simulates_spec2 vsp vsp' e
-      )
-*)
-let lemma_t_verify_simulates_spec (id:thread_id) (l:logS) 
-  : Lemma (requires (Valid? (t_verify id l)))
-          (ensures (vtls_rel (t_verify id l) (Spec.t_verify id (logS_to_logK id l))))
-  = admit()
-    //lemma_init_thread_state_rel id;
-    //lemma_t_verify_aux_simulates_spec (init_thread_state id) (Spec.init_thread_state id) l
 
 let rec lemma_get_log_to_state_op (vs:vtls) (l:logS{Valid? (fst (t_verify_aux vs l))})
   : Lemma (ensures (Seq.equal (to_state_op_logS l) 
@@ -634,11 +606,24 @@ let lemma_logS_to_logK_to_state_op (id:thread_id) (l:logS{Valid? (t_verify id l)
   : Lemma (ensures (Seq.equal (to_state_op_logS l) 
                               (Veritas.EAC.to_state_op_vlog (logS_to_logK id l))))
   = lemma_get_log_to_state_op (init_thread_state id) l
+*)
+
+
+let rec lemma_t_verify_aux_valid_implies_prefix_valid
+  (vs:vtls) (l:logS) (i:nat{i <= Seq.length l}):
+  Lemma (requires (Valid? (fst (t_verify_aux vs l))))
+        (ensures (Valid? (fst (t_verify_aux vs (prefix l i)))))
+        (decreases (Seq.length l))
+  = let n = Seq.length l in
+    if n > 0 && i < n - 1
+    then 
+      let lp = prefix l (n - 1) in
+      lemma_t_verify_aux_valid_implies_prefix_valid  vs lp i
 
 let lemma_tl_verifiable_implies_prefix_verifiable
   (tl:tl_verifiable_log) (i:nat{i <= tl_length tl}):
   Lemma (ensures (tl_verifiable (tl_prefix tl i)))
-  = admit()
+  = lemma_t_verify_aux_valid_implies_prefix_valid (init_thread_state (fst tl)) (snd tl) i
 
 let lemma_gl_verifiable_implies_prefix_verifiable
   (gl:gl_verifiable_log) (i:nat{i <= Seq.length gl}):
@@ -649,46 +634,14 @@ let lemma_gl_verifiable_implies_prefix_verifiable
       = assert(thread_log glp tid = thread_log gl tid) in
     Classical.forall_intro aux
 
-let lemma_verifiable_append1  (gl:SpecVG.verifiable_log) (l:logK{SpecVT.verifiable (Seq.length gl, l)})
-  : Lemma (SpecVG.verifiable (append1 gl l))
+let lemma_verifiable_append1  (gl:SpecG.verifiable_log) (l:logK{SpecT.verifiable (Seq.length gl, l)})
+  : Lemma (SpecG.verifiable (append1 gl l))
   = let gl' = append1 gl l in
     assert (Seq.length gl' = Seq.length gl + 1);
-    let aux (i:seq_index gl') : Lemma (SpecVT.verifiable (SpecVG.thread_log gl' i))
+    let aux (i:seq_index gl') : Lemma (SpecT.verifiable (SpecG.thread_log gl' i))
       = if i < Seq.length gl 
-        then assert (SpecVT.verifiable (SpecVG.thread_log gl i)) in
+        then assert (SpecT.verifiable (SpecG.thread_log gl i)) in
     Classical.forall_intro aux
-
-let rec glogS_to_logK_aux (gl:gl_verifiable_log{forall_is_map gl}) 
-  : Tot (gl':SpecVG.verifiable_log{Seq.length gl = Seq.length gl'})
-    (decreases (Seq.length gl))
-  = let n = Seq.length gl in
-    if n = 0 then Seq.empty
-    else (
-      let glp = prefix gl (n - 1) in
-      let e = Seq.index gl (n - 1) in
-      admit()
-      //lemma_t_verify_simulates_spec (n - 1) e;
-      //lemma_verifiable_append1 (glogS_to_logK_aux glp) (logS_to_logK (n - 1) e);
-      //append1 (glogS_to_logK_aux glp) (logS_to_logK (n - 1) e)
-    )
-
-let glogS_to_logK (gl:gl_verifiable_log{forall_is_map gl}) 
-  : gl':SpecVG.verifiable_log{Seq.length gl = Seq.length gl'}
-  = glogS_to_logK_aux gl
-
-let rec lemma_glogS_to_logK_aux (gl:gl_verifiable_log{forall_is_map gl}) (id:seq_index gl)
-  : Lemma (ensures Seq.index (glogS_to_logK gl) id = logS_to_logK id (Seq.index gl id))
-          (decreases (Seq.length gl))
-  = admit()
-    //let n = Seq.length gl in
-    //if n <> 0
-    //then if id < n - 1
-    //then let glp = prefix gl (n - 1) in
-    //     lemma_glogS_to_logK_aux glp id
-
-let lemma_glogS_to_logK (gl:gl_verifiable_log{forall_is_map gl}) (id:seq_index gl)
-  : Lemma (ensures Seq.index (glogS_to_logK gl) id = logS_to_logK id (Seq.index gl id))
-  = lemma_glogS_to_logK_aux gl id
 
 (*
 let lemma_prefix_verifiable_and_forall_is_map (gl:gl_verifiable_log{forall_is_map gl}) (i:seq_index gl)
@@ -708,7 +661,6 @@ let lemma_prefix_glogS_to_logK_comm (gl:verifiable_log{forall_is_map gl}) (i:seq
   : Lemma (ensures Seq.equal (prefix (glogS_to_logK gl) i) (glogS_to_logK (prefix gl i)))
           [SMTPat (prefix (glogS_to_logK gl) i)]
   = ()
-*)
 
 let rec hadd_equal_aux (gl:gl_verifiable_log{forall_is_map gl}) 
   : Lemma (ensures hadd gl = SpecVG.hadd (glogS_to_logK gl))
@@ -741,7 +693,7 @@ let rec hevict_equal_aux (gl:gl_verifiable_log{forall_is_map gl})
 let lemma_hevict_equal (gl:gl_verifiable_log{forall_is_map gl}) 
   : Lemma (hevict gl = SpecVG.hevict (glogS_to_logK gl))
   = hevict_equal_aux gl
-
+*)
 let clock_sorted (il: il_logS {il_verifiable il})
   = admit()
  
@@ -759,103 +711,123 @@ let il_create (gl: gl_verifiable_log): (itsl:its_log{g_logS_of itsl == gl})
 
 
 
-let thread_state (itsl:its_log)
-                 (tid:valid_tid itsl)
+let thread_state (il:its_log)
+                 (tid:valid_tid il)
   : Tot (vs:vtls{Valid? vs})
-  = verify (thread_log (I.s_seq itsl) tid)
+  = verify (thread_log (I.s_seq il) tid)
 
-let il_thread_id_of (itsl: its_log) (i: I.seq_index itsl): valid_tid itsl =
-  fst (I.i2s_map itsl i)
+let il_thread_id_of (il: its_log) (i: I.seq_index il): valid_tid il =
+  fst (I.i2s_map il i)
 
-let thread_state_pre (itsl: its_log) (i: I.seq_index itsl): (vs:vtls{Valid? vs}) = 
-  let tid = il_thread_id_of itsl i in
-  thread_state (I.prefix itsl i) tid
+let thread_state_pre (il: its_log) (i: I.seq_index il): (vs:vtls{Valid? vs}) = 
+  let tid = il_thread_id_of il i in
+  thread_state (I.prefix il i) tid
 
-let thread_state_post (itsl: its_log) (i: I.seq_index itsl): (vs:vtls{Valid? vs}) = 
-  let tid = il_thread_id_of itsl i in
-  thread_state (I.prefix itsl (i + 1)) tid
+let thread_state_post (il: its_log) (i: I.seq_index il): (vs:vtls{Valid? vs}) = 
+  let tid = il_thread_id_of il i in
+  thread_state (I.prefix il (i + 1)) tid
 
-let lemma_verifier_thread_state_extend (itsl: its_log) (i: I.seq_index itsl):
-  Lemma (thread_state_post itsl i == 
-         t_verify_step (thread_state_pre itsl i) (I.index itsl i))
-  = admit()
+let t_verify_aux_snoc (vs:vtls) (l:logS) (e:logS_entry)
+  : Lemma (ensures
+             fst (t_verify_aux vs (Seq.snoc l e)) ==
+             t_verify_step (fst (t_verify_aux vs l)) e)
+  = assert (prefix (Seq.snoc l e) (Seq.length l) `Seq.equal` l)
 
-let forall_store_inv (itsl:its_log)
-  = forall (tid:valid_tid itsl). store_inv (thread_store (thread_state itsl tid))
-  
-let forall_vtls_rel (itsl:its_log) (itsl':SpecVTS.its_log) 
-  = thread_count itsl = SpecVTS.thread_count itsl' /\
-    (forall (tid:valid_tid itsl). 
-       vtls_rel (thread_state itsl tid) 
-                (SpecVTS.thread_state itsl' tid))
+let lemma_verifier_thread_state_extend (il: its_log) (i: I.seq_index il):
+  Lemma (thread_state_post il i == 
+         t_verify_step (thread_state_pre il i) (I.index il i))
+  = let tid = il_thread_id_of il i in
+    let il_i = I.prefix il i in
+    let il_i1 = I.prefix il (i + 1) in
+    let logS_tid = Seq.index (I.s_seq il_i) tid in
+    let logS_tid1 = Seq.index (I.s_seq il_i1) tid in
+    I.lemma_prefix_snoc il i;
+    assert (logS_tid1 `Seq.equal` Seq.snoc logS_tid (I.index il i));
+    let init = init_thread_state tid in
+    let lhs = t_verify_aux init logS_tid1 in
+    let rhs = t_verify_step (fst (t_verify_aux init logS_tid)) (I.index il i) in
+    t_verify_aux_snoc init logS_tid (I.index il i)
 
-let ilogS_to_logK (il:its_log{forall_store_inv il}) : SpecVTS.its_log
+(* Re-defining some spec-level constructs over SpecVT.il_vlog instead of
+   SpecVT.its_log -- TODO: worth changing the types in the spec? *)
+   
+let spec_thread_id_of (il: SpecTS.il_vlog) (i: I.seq_index il) : SpecTS.valid_tid il =
+  fst (I.i2s_map il i)
+
+let spec_thread_state (il: SpecTS.il_vlog) (tid: SpecTS.valid_tid il) : Spec.vtls
+  = SpecT.verify (SpecG.thread_log (I.s_seq il) tid)
+
+let spec_thread_state_pre (il: SpecTS.il_vlog) (i: I.seq_index il) : Spec.vtls = 
+  let tid = spec_thread_id_of il i in
+  spec_thread_state (I.prefix il i) tid
+
+let spec_thread_state_post (il: SpecTS.il_vlog) (i: I.seq_index il): Spec.vtls = 
+  let tid = spec_thread_id_of il i in
+  spec_thread_state (I.prefix il (i + 1)) tid
+
+
+let ilogS_to_logK (il:its_log) : SpecTS.il_vlog
   = admit()
 
 // WANT: I.index (ilogS_to_logK itsl) i == 
 //       logS_to_logK_entry (thread_state_pre itsl i) (I.index itsl i) 
 
-let lemma_ilogS_to_logK_length (itsl:its_log{forall_store_inv itsl})
-  : Lemma (ensures I.length itsl = I.length (ilogS_to_logK itsl))
-          [SMTPat (I.length (ilogS_to_logK itsl))]
+let lemma_ilogS_to_logK_length (il:its_log)
+  : Lemma (ensures I.length il = I.length (ilogS_to_logK il))
+          [SMTPat (I.length (ilogS_to_logK il))]
   = admit()
 
-let lemma_ilogS_to_logK_thread_count (itsl:its_log{forall_store_inv itsl})
-  : Lemma (ensures thread_count itsl = SpecVTS.thread_count (ilogS_to_logK itsl))
-          [SMTPat (SpecVTS.thread_count (ilogS_to_logK itsl))]
+let lemma_ilogS_to_logK_thread_count (il:its_log)
+  : Lemma (ensures thread_count il = SpecTS.thread_count (ilogS_to_logK il))
+          [SMTPat (SpecTS.thread_count (ilogS_to_logK il))]
   = admit()
 
-// Also want a function that can take an il:its_log{forall_store_inv il} and an
-// entry e such that adding e produces a state where is_map=true, but may or may
-// not satisfy store_inv, and produces a SpecVTS.its_log
-// --> still need to figure out exactly how this relates to ilogS_to_logK
-let extend_spec_log 
-      (il:its_log{forall_store_inv il}) 
-      (tid:valid_tid il)
-      (e:logS_entry{let vs = t_verify_step (thread_state il tid) e in
-                    Valid? vs /\ is_map (thread_store vs)})
-  : SpecVTS.its_log
+// may also want: prefix (ilogS_to_logK il) i == ilogS_to_logK (prefix il i)
+
+let forall_store_inv (il:its_log)
+  = forall (i:I.seq_index il). 
+      store_inv (thread_store (thread_state_post il i))
+
+let lemma_forall_store_inv_specialize (il:its_log) (i:I.seq_index il)
+  : Lemma (requires (forall_store_inv (I.prefix il i)))
+          (ensures (store_inv (thread_store (thread_state_pre il i))))
+  = // let tid = il_thread_id_of il i
+    // Either entry i is the first entry processed by thread tid (in which case store_inv
+    // holds by the defn of init_thread_state), or tid previously processed entry j. By our
+    // assumption, store_inv must hold after processing entry j ==> store_inv holds before
+    // processing entry i.
+    admit()
+
+let lemma_forall_store_inv_extend (il:its_log) (i:I.seq_index il)
+  : Lemma (requires (forall_store_inv (I.prefix il i) /\ 
+                     store_inv (thread_store (thread_state_post il i))))
+          (ensures (forall_store_inv (I.prefix il (i + 1))))
   = admit()
 
-let lemma_forall_store_inv_specialize (itsl:its_log) (i:I.seq_index itsl)
-  : Lemma (requires (forall_store_inv (I.prefix itsl i)))
-          (ensures (let tid = il_thread_id_of itsl i in
-                    store_inv (thread_store (thread_state (I.prefix itsl i) tid))))
-  = ()
+let forall_vtls_rel (il:its_log) (il':SpecTS.il_vlog) 
+  = I.length il = I.length il' /\
+    (forall (i:I.seq_index il). 
+       vtls_rel (thread_state_post il i) (spec_thread_state_post il' i))
 
-let lemma_forall_store_inv_extend (itsl:its_log) (i:I.seq_index itsl)
-  : Lemma (requires (let tid = il_thread_id_of itsl i in
-                     forall_store_inv (I.prefix itsl i) /\ 
-                     store_inv (thread_store (thread_state (I.prefix itsl (i + 1)) tid))))
-          (ensures (forall_store_inv (I.prefix itsl (i + 1))))
+let lemma_forall_vtls_rel_specialize (il:its_log) (i:I.seq_index il)
+  : Lemma (requires (forall_vtls_rel (I.prefix il i) (ilogS_to_logK (I.prefix il i))))
+          (ensures (vtls_rel (thread_state_pre il i)
+                             (spec_thread_state_pre (ilogS_to_logK il) i)))
   = admit()
 
-//let lemma_forall_store_inv_prefix (itsl:its_log{forall_store_inv itsl}) (i:I.seq_index itsl)
-//  : Lemma (ensures (forall_store_inv (I.prefix itsl i)))
-//          [SMTPat (forall_store_inv (I.prefix itsl i))]
-//  = admit()
-
-let lemma_forall_vtls_rel_specialize (itsl:its_log) (i:I.seq_index itsl)
-  : Lemma (requires (forall_store_inv (I.prefix itsl i) /\ 
-                     forall_vtls_rel (I.prefix itsl i) (ilogS_to_logK (I.prefix itsl i))))
-          (ensures (let tid = il_thread_id_of itsl i in
-                    vtls_rel (thread_state (I.prefix itsl i) tid)
-                             (SpecVTS.thread_state (ilogS_to_logK (I.prefix itsl i)) tid)))
+let lemma_forall_vtls_rel_extend (il:its_log) (i:I.seq_index il)
+  : Lemma (requires (let il_i = I.prefix il i in
+                     forall_vtls_rel il_i (ilogS_to_logK il_i) /\
+                     vtls_rel (thread_state_post il i) 
+                              (spec_thread_state_post (ilogS_to_logK il) i)))
+          (ensures (forall_vtls_rel (I.prefix il (i + 1)) (I.prefix (ilogS_to_logK il) (i + 1))))
   = admit()
 
-let lemma_forall_vtls_rel_extend (itsl:its_log) (i:I.seq_index itsl)
-  : Lemma (requires (let tid = il_thread_id_of itsl i in
-                     let itsl_i = I.prefix itsl i in
-                     forall_store_inv itsl_i /\
-                     forall_vtls_rel itsl_i (ilogS_to_logK itsl_i) /\
-                     (let e = I.index itsl i in
-                      let vs = thread_state itsl_i tid in
-                      let vs1 = t_verify_step vs e in
-                       Valid? vs1 /\ is_map (thread_store vs1) /\
-                       vtls_rel vs1 (SpecVTS.thread_state (extend_spec_log itsl_i tid e) tid))))
-          (ensures (let tid = il_thread_id_of itsl i in
-                    let e = I.index itsl i in
-                    forall_vtls_rel (I.prefix itsl (i + 1)) (extend_spec_log (I.prefix itsl i) tid e)))
+let lemma_forall_vtls_rel_implies_its (il:its_log)
+  : Lemma (requires (forall_vtls_rel il (ilogS_to_logK il)))
+          (ensures (let il_k = ilogS_to_logK il in
+                    SpecTS.verifiable il_k /\ SpecTS.clock_sorted il_k))
+          [SMTPat (forall_vtls_rel il (ilogS_to_logK il))]
   = admit()
 
 (* property that:
@@ -863,15 +835,15 @@ let lemma_forall_vtls_rel_extend (itsl:its_log) (i:I.seq_index itsl)
  *    (b) the spec level log is evict-add-consistent 
  *    (c) the intermediate and spec level verifiers states correspond to one-another (related)
  *)
-let store_inv_spec_eac_rel (itsl: its_log) = 
-  forall_store_inv itsl /\
-  (let itsl_k = ilogS_to_logK itsl in
-   SpecVTS.is_eac itsl_k /\
-   forall_vtls_rel itsl itsl_k)
+let store_inv_spec_eac_rel (il: its_log) = 
+  let il_k = ilogS_to_logK il in
+  forall_store_inv il /\
+  forall_vtls_rel il il_k /\
+  SpecTS.is_eac il_k
 
 (* a union type that contains a hash collision or a proof of store_inv_spec_eac_rel for a specific itsl log *)
-let store_inv_spec_rel_or_hashcollision (itsl:its_log) = 
-  o:option Veritas.Verifier.EAC.hash_collision_gen{Some? o \/ store_inv_spec_eac_rel itsl}
+let store_inv_spec_rel_or_hashcollision (il:its_log) = 
+  o:option hash_collision_gen{Some? o \/ store_inv_spec_eac_rel il}
 
 let inductive_step (itsl: il_hash_verifiable_log) 
                    (i:I.seq_index itsl {let itsl_i = I.prefix itsl i in
@@ -882,21 +854,22 @@ let inductive_step (itsl: il_hash_verifiable_log)
   let itsl_i = I.prefix itsl i in
   let itsl_k_i = ilogS_to_logK itsl_i in
   let itsl_i1 = I.prefix itsl (i + 1) in
+  let itsl_k_i1 = ilogS_to_logK itsl_i1 in  
 
-  // assert (SpecVTS.is_eac itsl_k_i);
-  // assert (forall_store_inv itsl_i);
-  // assert (forall_vtls_rel itsl_i itsl_k_i);
-
+  assert (forall_store_inv itsl_i);
+  assert (forall_vtls_rel itsl_i itsl_k_i);
+  assert (SpecTS.is_eac itsl_k_i);
+  
   let vs = thread_state itsl_i tid in
-  let vs' = SpecVTS.thread_state itsl_k_i tid in 
+  let vs' = spec_thread_state itsl_k_i tid in 
 
   lemma_forall_store_inv_specialize itsl i;
-  // assert (store_inv (thread_store vs));
+  assert (store_inv (thread_store vs));
   lemma_forall_vtls_rel_specialize itsl i;
-  // assert (vtls_rel vs vs');
+  assert (vtls_rel vs vs');
 
   lemma_verifier_thread_state_extend itsl i;
-  //assert (thread_state_post itsl i == t_verify_step (thread_state_pre itsl i) (I.index itsl i));
+  assert (thread_state_post itsl i == t_verify_step (thread_state_pre itsl i) (I.index itsl i));
 
   let st = thread_store vs in
   let e = I.index itsl i in
@@ -905,29 +878,27 @@ let inductive_step (itsl: il_hash_verifiable_log)
   | Get_S s k v ->
     lemma_vget_simulates_spec vs vs' s k v;
 
-    let itsl_k_i1 = extend_spec_log itsl_i tid e in
-    if SpecVTS.is_eac itsl_k_i1 then (
+    if SpecTS.is_eac itsl_k_i1 then (
        lemma_vget_preserves_inv vs s k v;
        lemma_forall_store_inv_extend itsl i;
        lemma_forall_vtls_rel_extend itsl i;
        None
     )
     else 
-      Some (Veritas.Verifier.EAC.lemma_non_eac_get_implies_hash_collision itsl_k_i1)
+      Some (lemma_non_eac_get_implies_hash_collision itsl_k_i1)
 
   | Put_S s k v ->
     lemma_vput_simulates_spec vs vs' s k v;
 
-    let itsl_k_i1 = extend_spec_log itsl_i tid e in
-    if SpecVTS.is_eac itsl_k_i1 then (
+    if SpecTS.is_eac itsl_k_i1 then (
        lemma_vput_preserves_inv vs s k v; 
        lemma_forall_store_inv_extend itsl i;        
-       SpecVTS.lemma_verifier_thread_state_extend itsl_k_i1 i; 
+       SpecTS.lemma_verifier_thread_state_extend itsl_k_i1 i; 
        lemma_forall_vtls_rel_extend itsl i;
        None
     )
     else 
-      Some (Veritas.Verifier.EAC.lemma_non_eac_put_implies_hash_collision itsl_k_i1)
+      Some (lemma_non_eac_put_implies_hash_collision itsl_k_i1)
 
   | AddM_S s (k,v) s' ->
       if store_contains_key st k
@@ -944,8 +915,7 @@ let inductive_step (itsl: il_hash_verifiable_log)
         let k' = stored_key st s' in
         lemma_vaddm_simulates_spec_if_k_is_new vs vs' s s' (k,v) k';
         
-        let itsl_k_i1 = extend_spec_log itsl_i tid e in
-        if SpecVTS.is_eac itsl_k_i1 then (
+        if SpecTS.is_eac itsl_k_i1 then (
           
           // The following should hold from eac -- right?
           assume(no_other_slot_points_to st s' k);
@@ -959,7 +929,7 @@ let inductive_step (itsl: il_hash_verifiable_log)
           None
         )
         else 
-          Some (Veritas.Verifier.EAC.lemma_non_eac_addm_implies_hash_collision itsl_k_i1)      
+          Some (lemma_non_eac_addm_implies_hash_collision itsl_k_i1)      
       )
 
   (*
@@ -997,27 +967,31 @@ let rec lemma_il_hash_verifiable_implies_eac_and_vtls_rel_aux
         // assert(store_inv_spec_rel_or_hashcollision itsl_i');
         inductive_step itsl (i - 1)      
     
-let lemma_il_hash_verifiable_implies_eac_and_vtls_rel (itsl: il_hash_verifiable_log)
-  : store_inv_spec_rel_or_hashcollision itsl     
-  = I.lemma_fullprefix_equal itsl;
-    lemma_il_hash_verifiable_implies_eac_and_vtls_rel_aux itsl (I.length itsl)
+let lemma_il_hash_verifiable_implies_eac_and_vtls_rel (il: il_hash_verifiable_log)
+  : store_inv_spec_rel_or_hashcollision il     
+  = I.lemma_fullprefix_equal il;
+    lemma_il_hash_verifiable_implies_eac_and_vtls_rel_aux il (I.length il)
 
-let lemma_store_inv_spec_eac_rel_implies_spec_hash_verifiable (itsl:il_hash_verifiable_log)
-  : Lemma (requires store_inv_spec_eac_rel itsl)
-          (ensures SpecVTS.hash_verifiable (ilogS_to_logK itsl))
+let lemma_store_inv_spec_eac_rel_implies_spec_hash_verifiable (il:il_hash_verifiable_log)
+  : Lemma (requires store_inv_spec_eac_rel il)
+          (ensures SpecTS.hash_verifiable (ilogS_to_logK il))
   = admit()
 
+(*
+
+Commmented out for now -- need to change SpecTS.state_ops to take an il_vlog
+
 let lemma_ilogS_to_logK_state_ops (il:its_log{forall_store_inv il})
-  : Lemma (state_ops il == SpecVTS.state_ops (ilogS_to_logK il))
+  : Lemma (state_ops il == SpecTS.state_ops (ilogS_to_logK il))
   = admit()
 
 let lemma_time_seq_rw_consistent  
-  (itsl: il_hash_verifiable_log {~ (Veritas.State.rw_consistent (state_ops itsl))})
-  : Veritas.Verifier.EAC.hash_collision_gen = 
-  let tsl = I.i_seq itsl in  
+  (il: il_hash_verifiable_log {~ (rw_consistent (state_ops il))})
+  : hash_collision_gen = 
+  let tsl = I.i_seq il in  
   let ts_ops = to_state_op_logS tsl in
 
-  let hc_or_inv = lemma_il_hash_verifiable_implies_eac_and_vtls_rel itsl in
+  let hc_or_inv = lemma_il_hash_verifiable_implies_eac_and_vtls_rel il in
 
   (* if hc_or_inv returns a hash collision, then we can return the same collision *)
   if Some? hc_or_inv
@@ -1025,54 +999,54 @@ let lemma_time_seq_rw_consistent
 
   (* otherwise, we can use the spec-level lemma *)
   else (
-    assert (store_inv_spec_eac_rel itsl);
+    assert (store_inv_spec_eac_rel il);
     
-    let itsl_k = ilogS_to_logK itsl in
+    let il_k = ilogS_to_logK il in
 
-    lemma_store_inv_spec_eac_rel_implies_spec_hash_verifiable itsl;
-    assert (SpecVTS.hash_verifiable itsl_k);
+    lemma_store_inv_spec_eac_rel_implies_spec_hash_verifiable il;
+    assert (SpecTS.hash_verifiable il_k);
 
-    lemma_ilogS_to_logK_state_ops itsl;
-    assert (state_ops itsl == SpecVTS.state_ops itsl_k);
+    lemma_ilogS_to_logK_state_ops il;
+    assert (state_ops il == SpecTS.state_ops il_k);
 
-    Veritas.Verifier.Correctness.lemma_time_seq_rw_consistent itsl_k
+    Veritas.Verifier.Correctness.lemma_time_seq_rw_consistent il_k
   )
 
 let lemma_logS_interleave_implies_state_ops_interleave (l: logS) (gl: g_logS{I.interleave #logS_entry l gl})
-  : Lemma (I.interleave #Veritas.State.state_op (to_state_op_logS l) (to_state_op_glogS gl)) 
+  : Lemma (I.interleave #state_op (to_state_op_logS l) (to_state_op_glogS gl)) 
   = admit()
 
 (* final correctness lemma; essentially a copy-and-paste from Veritas.Verifier.Correctness *)
-let lemma_verifier_correct (gl: gl_hash_verifiable_log { ~ (Veritas.State.seq_consistent (to_state_op_glogS gl))})
-  : Veritas.Verifier.EAC.hash_collision_gen 
+let lemma_verifier_correct (gl: gl_hash_verifiable_log { ~ (seq_consistent (to_state_op_glogS gl))})
+  : hash_collision_gen 
   = (* sequences of per-thread put/get operations *)
     let g_ops = to_state_op_glogS gl in
 
     (* sequence ordered by time of each log entry *)
-    let itsl = il_create gl in  
-    I.lemma_interleaving_correct itsl;
-    assert(I.interleave (I.i_seq itsl) gl);
+    let il = il_create gl in  
+    I.lemma_interleaving_correct il;
+    assert(I.interleave (I.i_seq il) gl);
 
     (* sequence of state ops induced by tmsl *)
-    let ts_ops = state_ops itsl in
+    let ts_ops = state_ops il in
 
-    lemma_logS_interleave_implies_state_ops_interleave (I.i_seq itsl) gl;
+    lemma_logS_interleave_implies_state_ops_interleave (I.i_seq il) gl;
     assert(I.interleave ts_ops g_ops);
 
     (* if ts_ops is read-write consistent then we have a contradiction *)
-    let is_rw_consistent = Veritas.SeqMachine.valid_all_comp Veritas.StateSeqMachine.ssm ts_ops in
-    Veritas.StateSeqMachine.lemma_state_sm_equiv_rw_consistent ts_ops;
+    let is_rw_consistent = valid_all_comp ssm ts_ops in
+    lemma_state_sm_equiv_rw_consistent ts_ops;
 
     if is_rw_consistent then (
-      assert(Veritas.SeqMachine.valid_all Veritas.StateSeqMachine.ssm ts_ops);
-      assert(Veritas.State.rw_consistent ts_ops);
+      assert(valid_all ssm ts_ops);
+      assert(rw_consistent ts_ops);
 
       (* a contradiction *)
-      assert(Veritas.State.seq_consistent g_ops);
+      assert(seq_consistent g_ops);
 
       (* any return value *)
-      Veritas.Verifier.EAC.SingleHashCollision (Collision (DVal Null) (DVal Null))
+      SingleHashCollision (Collision (DVal Null) (DVal Null))
     )
     else  
-      lemma_time_seq_rw_consistent itsl
-
+      lemma_time_seq_rw_consistent il
+*)
